1. Use a correct condition in the `for` loop: separate conditions with a semicolon (`;`), not a comma.
2. To handle shifting 'a' to 'b' and 'z' to 'a', you can use modulo arithmetic to implement a circular shift.

Hereâ€™s an updated version of your code:

```cpp
class Solution {
public:
    bool canMakeSubsequence(string str1, string str2) {
        int j = 0;
        int str1Length = str1.length();
        int str2Length = str2.length();
        if (str1Length < str2Length) return false;

        for (int i = 0; i < str1Length && j < str2Length; i++) {
            char shiftedChar = (str1[i] == 'z') ? 'a' : str1[i] + 1;
            if (str1[i] == str2[j] || shiftedChar == str2[j]) {
                j++;
            }
        }

        return j == str2Length;
    }
};
```

### Explanation
1. **Loop Condition Correction:**
   - Change `for (int i = 0; i < str1Length, j < str2Length; i++)` to `for (int i = 0; i < str1Length && j < str2Length; i++)` to use `&&` for the condition.

2. **Character Shifting Logic:**
   - I added a variable `shiftedChar` to represent the character after the shift:
     - If `str1[i]` is `'z'`, it should wrap around to `'a'`.
     - Otherwise, simply add `1` to get the next character.

3. **Comparison Update:**
   - Now, we compare `str1[i]` directly to `str2[j]`, or `shiftedChar` to `str2[j]`.

This should solve your issue.

Instead of explicitly checking for the shifted character in every iteration, we can take advantage of modular arithmetic to simplify the comparison logic. This makes the solution more elegant and reduces the need for an additional variable.

Here is the updated version:

```cpp
class Solution {
public:
    bool canMakeSubsequence(string str1, string str2) {
        int j = 0;
        int str1Length = str1.length();
        int str2Length = str2.length();
        if (str1Length < str2Length) return false;

        for (int i = 0; i < str1Length && j < str2Length; i++) {
            // Check if character matches directly or after a shift.
            if (str1[i] == str2[j] || (str1[i] - 'a' + 1) % 26 + 'a' == str2[j]) {
                j++;
            }
        }

        return j == str2Length;
    }
};
```

### Improvements Explained
1. **Modulo Arithmetic:**
   - The expression `(str1[i] - 'a' + 1) % 26 + 'a'` is used to determine the next character after `str1[i]`.
   - It wraps around if `str1[i]` is `'z'`, directly producing `'a'`.
   - This eliminates the need for an additional `shiftedChar` variable and makes the condition more compact.

2. **Code Simplicity:**
   - The updated code is more concise and elegant. It relies on the `modulus` operation to wrap around from `'z'` to `'a'` without requiring explicit branching.

This solution has the same time complexity of O(n), where n is the length of `str1`, and it also requires O(1) extra space. However, the new solution is more readable and slightly more efficient due to reduced branching.